
<div style='overflow: hidden; white-space: nowrap; text-align: center'><hr style='display: inline-block; width: 40%;' />    <span style="color:deepskyblue; font-weight:900; letter-spacing: 2px">Section 3.7</span>    <hr style='display: inline-block; width: 40%' /></div>
<div style="text-align: center;  line-height: .75"><span style="color: deepskyblue; font-weight:900; letter-spacing: 2px; font-size: 12px">◦ THE CHAIN RULE ◦</span></div>

<span style="color: red; font-weight: 800">THEOREM 3.1</span> **The Chain Rule**
	Suppose $y = f(u)$ is differentiable at $u = g(x)$ $and u = g(x)$ is differentiable at $x$. The composite function $y = f(g(x))$ is differentiable at $x$, and its derivative can be expressed in two equivalent ways:
$$
	\frac{dy}{dx} = \frac{dy}{du}\cdot\frac{du}{dx}
$$
$$
	\frac{d}{dx} = (f(g(x))) = f'(u) \cdot g'(x)
$$

<span style="color: royalblue; font-weight: 800">PROCEDURE</span> **Using the Chain Rule**
	Assume the differentiable function $y = f(g(x))$ is given.
	**1.** Identify an outer function $f$ and an inner function $g$, and let $u = g(x)$.
	**2.** Replace $g(x)$ with $u$ to express $y$ in terms of $u$:
$$
	y = f(g(x)) \Rightarrow y = f(u)
$$

<span style="color: red; font-weight: 800">THEOREM 3.1</span> **Chain Rule for Powers**
	If $g$ is differentiable for all $x$ in its domain and $p$ is a rule number, then:
$$
	\frac{d}{dx}((g(x))^p) = p(g(x))^{p - 1}g'(x)
$$

<div style='overflow: hidden; white-space: nowrap; text-align: center'><hr style='display: inline-block; width: 40%;' />    <span style="color:deepskyblue; font-weight:900; letter-spacing: 2px">Section 3.8</span>    <hr style='display: inline-block; width: 40%' /></div>
<div style="text-align: center;  line-height: .75"><span style="color: deepskyblue; font-weight:900; letter-spacing: 2px; font-size: 12px">◦ IMPLICIT DIFFERENTIATION ◦</span></div>

- Implicit differentiation aims to find a single expression for the derivative *directly* from an equation without first solving for $y$.
 
<div style='overflow: hidden; white-space: nowrap; text-align: center'><hr style='display: inline-block; width: 40%;' />    <span style="color:deepskyblue; font-weight:900; letter-spacing: 2px">Section 3.9</span>    <hr style='display: inline-block; width: 40%' /></div>
<div style="text-align: center;  line-height: .75"><span style="color: deepskyblue; font-weight:900; letter-spacing: 2px; font-size: 12px">◦ DERIVATIVES OF LOGARITHMS AND EXPONENTIAL FUNCTIONS ◦</span></div>

**Inverse Properties for $e^x$ and $ln\;x$**
	  **1.**  $e^{ln\:x}$, for $x > 0$, and $ln(e^x) = x$, for all $x$.
	  **2.** $y = ln\;x$ if and only if $x = e^y$
	  **3.** For real numbers $x$ and $b > 0$, $b^x = e^{ln\;b^x} = e^{xln\;b}$

<span style="color: red; font-weight: 800">THEOREM 3.15</span> **Derivative of $ln\;x$**
$$
	\frac{d}{dx}(ln\:x) = \frac1x,\;for\;x > 0\;\;\;\;\;\frac{d}{dx}(ln\:|x|) = \frac1x,\;for\;x \neq 0
$$

<span style="color: red; font-weight: 800">THEOREM 3.16</span> **Derivative of $b^x$**
	If $b > 0$ and $b \neq 1$, then for all $x$,
$$
	\frac{d}{dx}(b^x) = b^x\;ln\:b
$$

<span style="color: red; font-weight: 800">THEOREM 3.17</span> **General Power Rule**
	For real numbers $p$ and for $x > 0$,
$$
	\frac{d}{dx}(x^p) = px^{p - 1}
$$
	Furthermore, if $u$ is a positive differentiable function on its domain, then
$$
	\frac{d}{dx}(u(x)^p) = p(u(x))^{p - 1} \;\cdot u'(x)
$$

<span style="color: red; font-weight: 800">THEOREM 3.18</span> **Derivative of $log_b\;x$**
	If $b > 0$ and $b \neq 1$, then
$$
	\frac{d}{dx}(log_b\:x) = \frac{1}{x\:ln\:b},\;for\;x > 0\;\;\;and\;\;\;\frac{d}{dx}(log_b\:|x|) = \frac{1}{x\:ln\:b},\;for\;x \neq 0
$$


<div style='overflow: hidden; white-space: nowrap; text-align: center'><hr style='display: inline-block; width: 40%;' />    <span style="color:deepskyblue; font-weight:900; letter-spacing: 2px">Section 3.10</span>    <hr style='display: inline-block; width: 40%' /></div>
<div style="text-align: center;  line-height: .75"><span style="color: deepskyblue; font-weight:900; letter-spacing: 2px; font-size: 12px">◦ DERIVATIVES OF INVERSE TRIGONOMETRIC FUNCTIONS ◦</span></div>

<span style="color: red; font-weight: 800">THEOREM 3.19</span> **Derivative of Inverse Sine**
$$
	\frac{d}{dx}(\sin^{-1}\:x) = \frac{1}{\sqrt{1 - x^2}},\;for\;-1 < x < 1
$$

<span style="color: red; font-weight: 800">THEOREM 3.20</span> **Derivatives of Inverse Trigonometric Functions**
$$
	\frac{d}{dx}(\sin^{-1}\:x) = \frac{1}{\sqrt{1 - x^2}}\;\;\;\;\;\;\frac{d}{dx}(\cos^{-1}x) = -\frac{1}{\sqrt{1 - x^2}},\;for\;-1 < x < 1
$$
$$
	\frac{d}{dx}(\tan^{-1}x) = \frac{1}{1 + x^2}\;\;\;\;\;\;\frac{d}{dx}(\cot^{-1}x) = \frac{1}{1 + x^2},\;for\;-1 < x < 1
$$
$$
	
$$

<div style='overflow: hidden; white-space: nowrap; text-align: center'><hr style='display: inline-block; width: 40%;' />    <span style="color:deepskyblue; font-weight:900; letter-spacing: 2px">Section 3.11</span>    <hr style='display: inline-block; width: 40%' /></div>
<div style="text-align: center;  line-height: .75"><span style="color: deepskyblue; font-weight:900; letter-spacing: 2px; font-size: 12px">◦ RELATED RATES ◦</span></div>


